re-structuring proof scripts in Ackermann sub-directory

theories/ordinals/Ackermann/LNN2LNT.v
@@ -1,4 +1,4 @@
-
+(******************************************************************************)
 Require Import Ensembles.
 Require Import Coq.Lists.List.
 Require Import Arith.
@@ -32,32 +32,26 @@ Fixpoint LNN2LNT_term (t : fol.Term LNN) : Term :=
 Definition LTFormula :=
   existH 2 (equal (Plus (var 0) (Succ (var 2))) (var 1)).
 
+
 Definition translateLT (ts : fol.Terms LNN (arity LNN (inl _ LT))) : Formula.
-simpl in ts.
-induction (consTerms _ _ ts).
-induction x as (a, b).
-induction (consTerms _ _ b).
-induction x as (a0, b0).
-set (x := LNN2LNT_term a) in *.
-set (y := LNN2LNT_term a0) in *.
-apply (subAllFormula LNT LTFormula).
-intro.
-induction H as [| H HrecH].
-exact x.
-induction H as [| H HrecH0].
-exact y.
-exact (var H).
+Proof.
+  simpl in ts; destruct  (consTerms _ _ ts) as [(a,b) p].
+  destruct  (consTerms _ _ b) as [(a0,b0) p0].
+  set (x := LNN2LNT_term a) in *.
+  set (y := LNN2LNT_term a0) in *.
+  apply (subAllFormula LNT LTFormula).
+  intro n; induction n as [| n Hrecn].
+  - exact x.
+  - induction n  as [| n0 HrecH0].
+    + exact y.
+    + exact (var n0).
 Defined.
 
-Lemma LNN2LNT_natToTerm :
- forall n : nat, LNN2LNT_term (natToTermLNN n) = natToTerm n.
+Lemma LNN2LNT_natToTerm (n:nat): LNN2LNT_term (natToTermLNN n) = natToTerm n.
 Proof.
-intros.
-induction n as [| n Hrecn].
-reflexivity.
-simpl in |- *.
-rewrite Hrecn.
-reflexivity.
+  induction n as [| n Hrecn].
+  - reflexivity.
+  - simpl; now rewrite Hrecn.
 Qed.
 
 Lemma translateLT1 :
@@ -70,23 +64,13 @@ Lemma translateLT1 :
        nat_rec (fun _ : nat => fol.Term LNT) (LNN2LNT_term a0)
          (fun (H1 : nat) (_ : fol.Term LNT) => var H1) H0) H).
 Proof.
-intros.
-unfold translateLT in |- *.
-induction (consTerms LNN 1 (Tcons LNN 1 a (Tcons LNN 0 a0 b0))).
-induction x as (a1, b).
-simpl in |- *.
-induction (consTerms LNN 0 b).
-induction x as (a2, b1).
-simpl in |- *.
-simpl in p.
-inversion p.
-assert (b = Tcons LNN 0 a0 b0).
-refine (inj_right_pair2 _ eq_nat_dec _ _ _ _ H1).
-rewrite H in p0.
-simpl in p0.
-inversion p0.
-clear H4 H3 H H1 H0.
-reflexivity.
+  intros a a0 b0; unfold translateLT.  
+  destruct (consTerms LNN 1 (Tcons LNN 1 a (Tcons LNN 0 a0 b0))) as [(a1, b) p].
+  simpl; destruct (consTerms LNN 0 b) as [(a2, b1) p0].
+  simpl in p; inversion p.
+  assert (b = Tcons LNN 0 a0 b0)
+    by refine (inj_right_pair2 _ eq_nat_dec _ _ _ _ H1).
+  rewrite H in p0; simpl in p0; inversion p0; reflexivity.
 Qed.
 
 Fixpoint LNN2LNT_formula (f : fol.Formula LNN) : Formula :=
@@ -103,403 +87,319 @@ Fixpoint LNN2LNT_formula (f : fol.Formula LNN) : Formula :=
   | fol.forallH v A => forallH v (LNN2LNT_formula A)
   end.
 
-Lemma LNN2LNT_or :
- forall a b : fol.Formula LNN,
- LNN2LNT_formula (fol.orH LNN a b) =
- orH (LNN2LNT_formula a) (LNN2LNT_formula b).
-Proof.
-reflexivity.
-Qed.
+Lemma LNN2LNT_or (a b : fol.Formula LNN):
+  LNN2LNT_formula (fol.orH LNN a b) =
+    orH (LNN2LNT_formula a) (LNN2LNT_formula b).
+Proof. reflexivity. Qed.
 
-Lemma LNN2LNT_and :
- forall a b : fol.Formula LNN,
+Lemma LNN2LNT_and (a b : fol.Formula LNN):
  LNN2LNT_formula (fol.andH LNN a b) =
  andH (LNN2LNT_formula a) (LNN2LNT_formula b).
-Proof.
-reflexivity.
-Qed.
+Proof. reflexivity. Qed.
 
-Lemma LNN2LNT_iff :
- forall a b : fol.Formula LNN,
+Lemma LNN2LNT_iff (a b : fol.Formula LNN):
  LNN2LNT_formula (fol.iffH LNN a b) =
- iffH (LNN2LNT_formula a) (LNN2LNT_formula b).
-Proof.
-reflexivity.
-Qed.
+   iffH (LNN2LNT_formula a) (LNN2LNT_formula b).
+Proof. reflexivity. Qed.
 
-Lemma LNN2LNT_exist :
- forall (v : nat) (a : fol.Formula LNN),
+Lemma LNN2LNT_exist (v : nat) (a : fol.Formula LNN) :
  LNN2LNT_formula (fol.existH LNN v a) = existH v (LNN2LNT_formula a).
-Proof.
-reflexivity.
-Qed.
+Proof. reflexivity. Qed.
 
-Lemma LNN2LNT_freeVarTerm :
- forall t : fol.Term LNN,
+Lemma LNN2LNT_freeVarTerm (t : fol.Term LNN):
  freeVarTerm LNT (LNN2LNT_term t) = freeVarTerm LNN t.
 Proof.
-intros.
-elim t using
- Term_Terms_ind
-  with
+  induction t using
+    Term_Terms_ind
+    with
     (P0 := fun (n : nat) (ts : fol.Terms LNN n) =>
-           freeVarTerms LNT n (LNN2LNT_terms n ts) = freeVarTerms LNN n ts).
-intros.
-reflexivity.
-intros.
-simpl in |- *.
-repeat rewrite freeVarTermApply.
-apply H.
-reflexivity.
-intros.
-simpl in |- *.
-transitivity (freeVarTerm LNN t0 ++ freeVarTerms LNN n t1).
-rewrite <- H0.
-rewrite <- H.
-reflexivity.
-reflexivity.
+             freeVarTerms LNT n (LNN2LNT_terms n ts) = freeVarTerms LNN n ts).
+  - intros; reflexivity.
+  - intros; simpl; repeat rewrite freeVarTermApply; now apply IHt.
+  - intros; simpl; reflexivity. 
+  - transitivity (freeVarTerm LNN t ++ freeVarTerms LNN n t0).
+    + rewrite <- IHt0; rewrite <- IHt; reflexivity.
+    + reflexivity.
 Qed.
 
-Lemma LNN2LNT_freeVarTerms :
- forall (n : nat) (ts : fol.Terms LNN n),
- freeVarTerms LNT n (LNN2LNT_terms n ts) = freeVarTerms LNN n ts.
+Lemma LNN2LNT_freeVarTerms (n : nat) (ts : fol.Terms LNN n):
+    freeVarTerms LNT n (LNN2LNT_terms n ts) = freeVarTerms LNN n ts.
 Proof.
-intros.
-induction ts as [| n t ts Hrects].
-reflexivity.
-intros.
-simpl in |- *.
-transitivity (freeVarTerm LNN t ++ freeVarTerms LNN n ts).
-rewrite <- Hrects.
-rewrite <- LNN2LNT_freeVarTerm.
-reflexivity.
-reflexivity.
+  induction ts as [| n t ts Hrects].
+  - reflexivity.
+  - simpl; transitivity (freeVarTerm LNN t ++ freeVarTerms LNN n ts).
+    + rewrite <- Hrects; rewrite <- LNN2LNT_freeVarTerm; reflexivity.
+    + reflexivity.
 Qed.
 
-Lemma LNN2LNT_freeVarFormula :
- forall (f : fol.Formula LNN) (v : nat),
- In v (freeVarFormula LNT (LNN2LNT_formula f)) <->
+Lemma LNN2LNT_freeVarFormula (f : fol.Formula LNN) (v : nat):
+  In v (freeVarFormula LNT (LNN2LNT_formula f)) <->
+    In v (freeVarFormula LNN f).
+Proof.
+  induction f as [t t0| r t| f1 Hrecf1 f0 Hrecf0| f Hrecf| n f Hrecf].
+  - simpl; repeat rewrite LNN2LNT_freeVarTerm; tauto.
+  - destruct r. (* is LT *)
+    simpl. 
+    destruct (consTerms _ _ t) as [(a,b) p].
+    simpl in p; rewrite <- p.
+    destruct (consTerms _ _ b) as [(a0, b0) p0].
+    simpl in p0; rewrite <- p0.
+    rewrite translateLT1.
+    rewrite <- (nilTerms _ b0).
+    unfold freeVarTerms in |- *.
+    fold (freeVarTerm LNN) in |- *.
+    rewrite <- app_nil_end.
+    split.
+    + intros H; decompose record (freeVarSubAllFormula1 _ _ _ _ H).
+      destruct H1 as [H0| H0].
+      * rewrite <- H0 in H2.
+        simpl in H2.
+        rewrite LNN2LNT_freeVarTerm in H2.
+        auto with datatypes.
+      * destruct H0 as [H0| H0].
+        -- rewrite <- H0 in H2.
+           simpl in H2.
+           rewrite LNN2LNT_freeVarTerm in H2.
+           auto with datatypes.
+        -- contradiction.
+    + intro H; destruct (in_app_or _ _ _ H) as [H0 | H0].
+      * eapply freeVarSubAllFormula2.
+        simpl in |- *.
+        left.
+        reflexivity.
+        simpl in |- *.
+        rewrite LNN2LNT_freeVarTerm.
+        auto.
+      * eapply freeVarSubAllFormula2.
+        simpl in |- *.
+        right.
+        left.
+        reflexivity.
+        simpl in |- *.
+        rewrite LNN2LNT_freeVarTerm.
+        auto.
+  - simpl in |- *.
+    induction Hrecf1 as (H, H0).
+    induction Hrecf0 as (H1, H2).
+    split.
+    + intros H3; apply in_or_app.
+      destruct (in_app_or _ _ _ H3); tauto.
+    + intros H3; apply in_or_app.
+      destruct (in_app_or _ _ _ H3); tauto.
+  - assumption.
+  - simpl in |- *.
+    induction Hrecf as (H, H0).
+    split.
+    + intros H1; apply In_list_remove3.  
+      * apply H; eapply In_list_remove1; apply H1.
+      * eapply In_list_remove2; apply H1.
+    + intros H1; apply In_list_remove3.
+      * apply H0.
+        eapply In_list_remove1, H1.
+      * eapply In_list_remove2, H1.
+Qed.
+
+Lemma LNN2LNT_freeVarFormula1 (f : fol.Formula LNN) (v : nat):
+ In v (freeVarFormula LNT (LNN2LNT_formula f)) -> 
  In v (freeVarFormula LNN f).
 Proof.
-intros.
-induction f as [t t0| r t| f1 Hrecf1 f0 Hrecf0| f Hrecf| n f Hrecf].
-simpl in |- *.
-repeat rewrite LNN2LNT_freeVarTerm.
-tauto.
-induction r.
-simpl in |- *.
-induction (consTerms _ _ t).
-induction x as (a, b).
-simpl in p.
-rewrite <- p.
-induction (consTerms _ _ b).
-induction x as (a0, b0).
-simpl in p0.
-rewrite <- p0.
-rewrite translateLT1.
-rewrite <- (nilTerms _ b0).
-unfold freeVarTerms in |- *.
-fold (freeVarTerm LNN) in |- *.
-rewrite <- app_nil_end.
-split.
-intros.
-decompose record (freeVarSubAllFormula1 _ _ _ _ H).
-simpl in H1.
-induction H1 as [H0| H0].
-rewrite <- H0 in H2.
-simpl in H2.
-rewrite LNN2LNT_freeVarTerm in H2.
-auto with datatypes.
-induction H0 as [H0| H0].
-rewrite <- H0 in H2.
-simpl in H2.
-rewrite LNN2LNT_freeVarTerm in H2.
-auto with datatypes.
-contradiction.
-intros.
-induction (in_app_or _ _ _ H).
-eapply freeVarSubAllFormula2.
-simpl in |- *.
-left.
-reflexivity.
-simpl in |- *.
-rewrite LNN2LNT_freeVarTerm.
-auto.
-eapply freeVarSubAllFormula2.
-simpl in |- *.
-right.
-left.
-reflexivity.
-simpl in |- *.
-rewrite LNN2LNT_freeVarTerm.
-auto.
-simpl in |- *.
-induction Hrecf1 as (H, H0).
-induction Hrecf0 as (H1, H2).
-split.
-intros.
-apply in_or_app.
-induction (in_app_or _ _ _ H3); tauto.
-intros.
-apply in_or_app.
-induction (in_app_or _ _ _ H3); tauto.
-assumption.
-simpl in |- *.
-induction Hrecf as (H, H0).
-split.
-intros.
-apply In_list_remove3.
-apply H.
-eapply In_list_remove1.
-apply H1.
-eapply In_list_remove2.
-apply H1.
-intros.
-apply In_list_remove3.
-apply H0.
-eapply In_list_remove1.
-apply H1.
-eapply In_list_remove2.
-apply H1.
+  intros ?; destruct (LNN2LNT_freeVarFormula f v); auto.
 Qed.
 
-Lemma LNN2LNT_freeVarFormula1 :
- forall (f : fol.Formula LNN) (v : nat),
- In v (freeVarFormula LNT (LNN2LNT_formula f)) -> In v (freeVarFormula LNN f).
+Lemma LNN2LNT_freeVarFormula2 (f : fol.Formula LNN) (v : nat):
+  In v (freeVarFormula LNN f) -> 
+  In v (freeVarFormula LNT (LNN2LNT_formula f)).
 Proof.
-intros.
-induction (LNN2LNT_freeVarFormula f v).
-auto.
+intros ? ; destruct (LNN2LNT_freeVarFormula f v); auto.
 Qed.
 
-Lemma LNN2LNT_freeVarFormula2 :
- forall (f : fol.Formula LNN) (v : nat),
- In v (freeVarFormula LNN f) -> In v (freeVarFormula LNT (LNN2LNT_formula f)).
-Proof.
-intros.
-induction (LNN2LNT_freeVarFormula f v).
-auto.
-Qed.
-
-Lemma LNN2LNT_subTerm :
- forall (t : fol.Term LNN) (v : nat) (s : fol.Term LNN),
+Lemma LNN2LNT_subTerm (t : fol.Term LNN) (v : nat) (s : fol.Term LNN):
  LNN2LNT_term (substituteTerm LNN t v s) =
  substituteTerm LNT (LNN2LNT_term t) v (LNN2LNT_term s).
 Proof.
-intros.
-elim t using
- Term_Terms_ind
-  with
+  elim t using  Term_Terms_ind
+    with
     (P0 := fun (n : nat) (ts : fol.Terms LNN n) =>
-           LNN2LNT_terms n (substituteTerms LNN n ts v s) =
-           substituteTerms LNT n (LNN2LNT_terms n ts) v (LNN2LNT_term s)).
-intros.
-simpl in |- *.
-induction (eq_nat_dec v n); auto.
-simpl in |- *.
-intros.
-rewrite H.
-reflexivity.
-reflexivity.
-simpl in |- *.
-intros.
-rewrite H.
-rewrite H0.
-reflexivity.
+             LNN2LNT_terms n (substituteTerms LNN n ts v s) =
+               substituteTerms LNT n (LNN2LNT_terms n ts) v 
+                 (LNN2LNT_term s)).
+  - intros n; simpl; destruct (eq_nat_dec v n); auto.
+  - simpl in |- *; intros f t0 H; now rewrite H.
+  - reflexivity.
+  - intros n t0 H t1 H0; simpl; now rewrite H, H0. 
 Qed.
 
-Lemma LNN2LNT_subTerms :
- forall (n : nat) (ts : fol.Terms LNN n) (v : nat) (s : fol.Term LNN),
- LNN2LNT_terms n (substituteTerms LNN n ts v s) =
- substituteTerms LNT n (LNN2LNT_terms n ts) v (LNN2LNT_term s).
+Lemma LNN2LNT_subTerms 
+  (n : nat) (ts : fol.Terms LNN n) (v : nat) (s : fol.Term LNN):
+  LNN2LNT_terms n (substituteTerms LNN n ts v s) =
+    substituteTerms LNT n (LNN2LNT_terms n ts) v (LNN2LNT_term s).
 Proof.
-intros.
-induction ts as [| n t ts Hrects].
-reflexivity.
-simpl in |- *.
-rewrite Hrects.
-rewrite LNN2LNT_subTerm.
-reflexivity.
+  induction ts as [| n t ts Hrects].
+  - reflexivity.
+  - simpl; now rewrite Hrects,  LNN2LNT_subTerm.
 Qed.
 
-Lemma LNN2LNT_subFormula :
- forall (T : System) (f : fol.Formula LNN) (v : nat) (s : fol.Term LNN),
+(** still fragile proof. Use libhyps *)
+
+Lemma LNN2LNT_subFormula 
+ (T : System) (f : fol.Formula LNN) (v : nat) (s : fol.Term LNN):
  SysPrf T
    (iffH (LNN2LNT_formula (substituteFormula LNN f v s))
       (substituteFormula LNT (LNN2LNT_formula f) v (LNN2LNT_term s))).
 Proof.
-intros.
-apply sysExtend with (Empty_set Formula).
-unfold Included in |- *.
-intros.
-induction H.
-generalize f v s.
-clear T f v s.
-intro.
-elim f using Formula_depth_ind2; intros.
-simpl in |- *.
-rewrite (subFormulaEqual LNT).
-repeat rewrite LNN2LNT_subTerm.
-apply iffRefl.
-induction r.
-rewrite subFormulaRelation.
-simpl in |- *.
-induction (consTerms _ _ t).
-induction x as (a, b).
-simpl in p.
-rewrite <- p.
-induction (consTerms _ _ b).
-induction x as (a0, b0).
-simpl in p0.
-rewrite <- p0.
-rewrite translateLT1.
-apply iffSym.
-eapply iffTrans.
-apply (subSubAllFormula LNT).
-rewrite <- (nilTerms _ b0).
-replace
- (substituteTerms LNN 2 (Tcons LNN 1 a (Tcons LNN 0 a0 (Tnil LNN))) v s) with
- (Tcons LNN 1 (substituteTerm LNN a v s)
-    (Tcons LNN 0 (substituteTerm LNN a0 v s) (Tnil LNN))).
-rewrite translateLT1.
-rewrite
- (subAllFormula_ext LNT LTFormula
-    (fun H : nat =>
-     nat_rec (fun _ : nat => fol.Term LNT)
-       (LNN2LNT_term (substituteTerm LNN a v s))
-       (fun (H0 : nat) (_ : fol.Term LNT) =>
-        nat_rec (fun _ : nat => fol.Term LNT)
-          (LNN2LNT_term (substituteTerm LNN a0 v s))
-          (fun (H1 : nat) (_ : fol.Term LNT) => var H1) H0) H)
-    (fun n : nat =>
-     substituteTerm LNT
-       (nat_rec (fun _ : nat => fol.Term LNT) (LNN2LNT_term a)
-          (fun (H0 : nat) (_ : fol.Term LNT) =>
-           nat_rec (fun _ : nat => fol.Term LNT) (LNN2LNT_term a0)
-             (fun (H1 : nat) (_ : fol.Term LNT) => var H1) H0) n) v
-       (LNN2LNT_term s))).
-apply iffRefl.
-intros.
-destruct m as [| n].
-simpl in |- *.
-apply LNN2LNT_subTerm.
-destruct n.
-simpl in |- *.
-apply LNN2LNT_subTerm.
-simpl in H.
-decompose sum H.
-discriminate H0.
-discriminate H1.
-reflexivity.
-rewrite subFormulaImp.
-simpl in |- *.
-rewrite (subFormulaImp LNT).
-apply (reduceImp LNT).
-apply H.
-apply H0.
-rewrite subFormulaNot.
-simpl in |- *.
-rewrite (subFormulaNot LNT).
-apply (reduceNot LNT).
-apply H.
-simpl in |- *.
-decompose record (subFormulaForall2 LNN a v v0 s).
-rewrite H4; clear H4.
-decompose record
- (subFormulaForall2 LNT (LNN2LNT_formula a) v v0 (LNN2LNT_term s)).
-unfold forallH in |- *.
-rewrite H7; clear H7.
-induction (eq_nat_dec v v0).
-simpl in |- *.
-apply iffRefl.
-simpl in |- *.
-apply
- iffTrans
-  with
-    (forallH x0
-       (substituteFormula LNT
-          (LNN2LNT_formula
-             (substituteFormula LNN
-                (substituteFormula LNN a v (fol.var LNN x)) v0 s)) x 
-          (var x0))).
-apply (rebindForall LNT).
-unfold not in |- *; intros.
-assert
- (In x0
-    (freeVarFormula LNT
-       (LNN2LNT_formula
-          (substituteFormula LNN (substituteFormula LNN a v (fol.var LNN x))
-             v0 s)))).
-eapply In_list_remove1.
-apply H6.
-assert
- (In x0
-    (freeVarFormula LNN
-       (substituteFormula LNN (substituteFormula LNN a v (fol.var LNN x)) v0
-          s))).
-apply LNN2LNT_freeVarFormula1.
-assumption.
-induction (freeVarSubFormula3 _ _ _ _ _ H8).
-assert
- (In x0 (freeVarFormula LNN (substituteFormula LNN a v (fol.var LNN x)))).
-eapply In_list_remove1.
-apply H9.
-induction (freeVarSubFormula3 _ _ _ _ _ H10).
-elim H5.
-eapply In_list_remove3.
-apply LNN2LNT_freeVarFormula2.
-eapply In_list_remove1.
-apply H11.
-eapply In_list_remove2.
-apply H11.
-elim (In_list_remove2 _ _ _ _ _ H6).
-induction H11 as [H11| H11].
-auto.
-contradiction.
-elim H4.
-rewrite LNN2LNT_freeVarTerm.
-assumption.
-apply (reduceForall LNT).
-apply (notInFreeVarSys LNT).
-apply
- iffTrans
-  with
-    (substituteFormula LNT
-       (substituteFormula LNT
-          (substituteFormula LNT (LNN2LNT_formula a) v (fol.var LNT x)) v0
-          (LNN2LNT_term s)) x (var x0)).
-apply (reduceSub LNT).
-apply (notInFreeVarSys LNT).
-eapply iffTrans.
-apply H.
-eapply eqDepth.
-symmetry  in |- *; rewrite subFormulaDepth; symmetry  in |- *. (*Hack to rewrite the right occ*)
-reflexivity.
-apply depthForall.
-apply (reduceSub LNT).
-apply (notInFreeVarSys LNT).
-eapply iffTrans.
-apply H.
-apply depthForall.
-simpl in |- *.
-apply iffRefl.
-eapply iffTrans.
-apply (subFormulaExch LNT).
-auto.
-rewrite LNN2LNT_freeVarTerm.
-auto.
-simpl in |- *.
-tauto.
-apply (reduceSub LNT).
-apply (notInFreeVarSys LNT).
-apply (subFormulaTrans LNT).
-unfold not in |- *; intros; elim H2.
-apply In_list_remove3.
-apply LNN2LNT_freeVarFormula1.
-eapply In_list_remove1.
-apply H6.
-eapply In_list_remove2.
-apply H6.
+  apply sysExtend with (Empty_set Formula).
+  -  intros x H; destruct H.
+  - generalize f v s; clear T f v s; intro f.
+    elim f using Formula_depth_ind2; intros.
+    + simpl; rewrite (subFormulaEqual LNT).
+      repeat rewrite LNN2LNT_subTerm; apply iffRefl.
+    + induction r.
+      rewrite subFormulaRelation; simpl.
+      destruct (consTerms _ _ t) as [(a,b) p].
+      simpl in p; rewrite <- p.
+      destruct (consTerms _ _ b) as [(a0,b0) p0].
+      simpl in p0; rewrite <- p0.
+      rewrite translateLT1.
+      apply iffSym; eapply iffTrans.
+      * apply (subSubAllFormula LNT).
+      * rewrite <- (nilTerms _ b0).
+        replace
+          (substituteTerms LNN 2 (Tcons _ 1 a (Tcons _ 0 a0 (Tnil _))) v s) 
+          with
+          (Tcons LNN 1 (substituteTerm _ a v s)
+             (Tcons _ 0 (substituteTerm _ a0 v s) (Tnil _))).
+        rewrite translateLT1.
+        rewrite
+          (subAllFormula_ext LNT LTFormula
+             (fun H : nat =>
+                nat_rec (fun _ : nat => fol.Term LNT)
+                  (LNN2LNT_term (substituteTerm LNN a v s))
+                  (fun (H0 : nat) (_ : fol.Term LNT) =>
+                     nat_rec (fun _ : nat => fol.Term LNT)
+                       (LNN2LNT_term (substituteTerm LNN a0 v s))
+                       (fun (H1 : nat) (_ : fol.Term LNT) => var H1) H0) H)
+             (fun n : nat =>
+                substituteTerm LNT
+                  (nat_rec (fun _ : nat => fol.Term LNT) (LNN2LNT_term a)
+                     (fun (H0 : nat) (_ : fol.Term LNT) =>
+                        nat_rec (fun _ : nat => fol.Term LNT) (LNN2LNT_term a0)
+                          (fun (H1 : nat) (_ : fol.Term LNT) => var H1) H0) n) v
+                  (LNN2LNT_term s))).
+        -- apply iffRefl.
+        -- intros m H; destruct m as [| n].
+           ++ simpl; apply LNN2LNT_subTerm.
+           ++ destruct n as [| n].
+              ** simpl in |- *.
+                 apply LNN2LNT_subTerm.
+              ** simpl in H.
+                 decompose sum H.
+                 discriminate H0.
+                 discriminate H1.
+        -- reflexivity.
+    + rewrite subFormulaImp; simpl.
+      rewrite (subFormulaImp LNT).
+      apply (reduceImp LNT).
+      apply H.
+      apply H0.
+    + rewrite subFormulaNot.
+      simpl; rewrite (subFormulaNot LNT).
+      apply (reduceNot LNT).
+      apply H.
+    + simpl; decompose record (subFormulaForall2 LNN a v v0 s).
+      rewrite H4; clear H4.
+      decompose record
+        (subFormulaForall2 LNT (LNN2LNT_formula a) v v0 (LNN2LNT_term s)).
+      unfold forallH in |- *.
+      rewrite H7; clear H7.
+      destruct (eq_nat_dec v v0) as [e | ].
+      * simpl; apply iffRefl.
+      * simpl; apply iffTrans with
+          (forallH x0
+             (substituteFormula LNT
+                (LNN2LNT_formula
+                   (substituteFormula LNN
+                      (substituteFormula LNN a v (fol.var LNN x)) v0 s)) x 
+                (var x0))).
+        apply (rebindForall LNT).
+        intros H6. 
+        assert
+          (H7: In x0
+             (freeVarFormula LNT
+                (LNN2LNT_formula
+                   (substituteFormula LNN
+                      (substituteFormula LNN a v (fol.var LNN x))
+                      v0 s))))
+          by (eapply In_list_remove1; apply H6). 
+        assert
+          (H8: In x0
+                 (freeVarFormula LNN
+                    (substituteFormula LNN (substituteFormula LNN a v 
+                                              (fol.var LNN x)) v0
+                       s)))
+          by (apply LNN2LNT_freeVarFormula1; assumption).
+        induction (freeVarSubFormula3 _ _ _ _ _ H8).
+        assert
+          (H10: In x0 (freeVarFormula LNN 
+                         (substituteFormula LNN a v (fol.var LNN x)))) 
+          by (eapply In_list_remove1; apply H9).
+        induction (freeVarSubFormula3 _ _ _ _ _ H10).
+        elim H5.
+        eapply In_list_remove3.
+        apply LNN2LNT_freeVarFormula2.
+        eapply In_list_remove1.
+        apply H11.
+        eapply In_list_remove2.
+        apply H11.
+        elim (In_list_remove2 _ _ _ _ _ H6).
+        destruct H11 as [H11| H11].
+        -- auto.
+        -- contradiction.
+        -- elim H4.
+        rewrite LNN2LNT_freeVarTerm.
+        assumption.
+        -- apply (reduceForall LNT).
+           apply (notInFreeVarSys LNT).
+           apply
+             iffTrans
+             with
+             (substituteFormula LNT
+                (substituteFormula LNT
+                   (substituteFormula LNT (LNN2LNT_formula a) v 
+                      (fol.var LNT x)) v0
+                   (LNN2LNT_term s)) x (var x0)).
+           apply (reduceSub LNT).
+           apply (notInFreeVarSys LNT).
+           eapply iffTrans.
+           apply H.
+           eapply eqDepth.
+           symmetry  in |- *; rewrite subFormulaDepth; 
+             symmetry  in |- *. (*Hack to rewrite the right occ*)
+           reflexivity.
+           apply depthForall.
+           apply (reduceSub LNT).
+           apply (notInFreeVarSys LNT).
+           eapply iffTrans.
+           apply H.
+           apply depthForall.
+           simpl in |- *.
+           apply iffRefl.
+           eapply iffTrans.
+           apply (subFormulaExch LNT).
+           auto.
+           rewrite LNN2LNT_freeVarTerm.
+           auto.
+           simpl in |- *.
+           tauto.
+           apply (reduceSub LNT).
+           apply (notInFreeVarSys LNT).
+           apply (subFormulaTrans LNT).
+           unfold not in |- *; intros; elim H2.
+           apply In_list_remove3.
+           apply LNN2LNT_freeVarFormula1.
+           eapply In_list_remove1.
+           apply H6.
+           eapply In_list_remove2.
+           apply H6.
 Qed.
 
 Fixpoint LNT2LNN_term (t : Term) : fol.Term LNN :=
@@ -515,15 +415,12 @@ Fixpoint LNT2LNN_term (t : Term) : fol.Term LNN :=
   | Tcons m s ss => Tcons LNN m (LNT2LNN_term s) (LNT2LNN_terms m ss)
   end.
 
-Lemma LNT2LNN_natToTerm :
- forall n : nat, LNT2LNN_term (natToTerm n) = natToTermLNN n.
+Lemma LNT2LNN_natToTerm (n:  nat) :
+  LNT2LNN_term (natToTerm n) = natToTermLNN n.
 Proof.
-intros.
-induction n as [| n Hrecn].
-reflexivity.
-simpl in |- *.
-rewrite Hrecn.
-reflexivity.
+  induction n as [| n Hrecn].
+  - reflexivity.
+  - simpl; now rewrite Hrecn.
 Qed.
 
 Fixpoint LNT2LNN_formula (f : Formula) : fol.Formula LNN :=
@@ -536,152 +433,113 @@ Fixpoint LNT2LNN_formula (f : Formula) : fol.Formula LNN :=
   | fol.forallH v A => fol.forallH LNN v (LNT2LNN_formula A)
   end.
 
-Lemma LNT2LNT_term : forall t : Term, LNN2LNT_term (LNT2LNN_term t) = t.
+Lemma LNT2LNT_term (t : Term): LNN2LNT_term (LNT2LNN_term t) = t.
 Proof.
-intros.
-elim t using
- Term_Terms_ind
-  with
+  elim t using
+    Term_Terms_ind
+    with
     (P0 := fun (n : nat) (ts : fol.Terms LNT n) =>
-           LNN2LNT_terms n (LNT2LNN_terms n ts) = ts); 
- simpl in |- *; intros.
-reflexivity.
-rewrite H.
-reflexivity.
-reflexivity.
-rewrite H.
-rewrite H0.
-reflexivity.
+             LNN2LNT_terms n (LNT2LNN_terms n ts) = ts); 
+    simpl in |- *.
+  - reflexivity.
+  - intros f t0 H; now rewrite H.
+  - reflexivity.
+  - intros n t0 H t1 H0. now rewrite H, H0.
 Qed.
 
-Lemma LNT2LNT_formula :
- forall f : Formula, LNN2LNT_formula (LNT2LNN_formula f) = f.
+Lemma LNT2LNT_formula (f : Formula): 
+ LNN2LNT_formula (LNT2LNN_formula f) = f.
 Proof.
-intros.
-induction f as [t t0| r t| f1 Hrecf1 f0 Hrecf0| f Hrecf| n f Hrecf];
- simpl in |- *.
-repeat rewrite LNT2LNT_term.
-reflexivity.
-induction r.
-rewrite Hrecf1.
-rewrite Hrecf0.
-reflexivity.
-rewrite Hrecf.
-reflexivity.
-rewrite Hrecf.
-reflexivity.
+  induction f as [t t0| r t| f1 Hrecf1 f0 Hrecf0| f Hrecf| n f Hrecf];
+    simpl.
+- now repeat rewrite LNT2LNT_term.
+- destruct r.
+- now rewrite Hrecf1, Hrecf0.
+- now rewrite Hrecf.
+- now rewrite Hrecf.
 Qed.
 
-Lemma LNT2LNN_subTerm :
- forall (t : Term) (v : nat) (s : Term),
- LNT2LNN_term (substituteTerm LNT t v s) =
- substituteTerm LNN (LNT2LNN_term t) v (LNT2LNN_term s).
+Lemma LNT2LNN_subTerm  (t : Term) (v : nat) (s : Term):
+  LNT2LNN_term (substituteTerm LNT t v s) =
+    substituteTerm LNN (LNT2LNN_term t) v (LNT2LNN_term s).
 Proof.
-intros.
-elim t using
- Term_Terms_ind
-  with
+  elim t using
+    Term_Terms_ind
+    with
     (P0 := fun (n : nat) (ts : fol.Terms LNT n) =>
-           LNT2LNN_terms n (substituteTerms LNT n ts v s) =
-           substituteTerms LNN n (LNT2LNN_terms n ts) v (LNT2LNN_term s));
- simpl in |- *; intros.
-induction (eq_nat_dec v n).
-reflexivity.
-reflexivity.
-rewrite H.
-reflexivity.
-reflexivity.
-rewrite H.
-rewrite H0.
-reflexivity.
+             LNT2LNN_terms n (substituteTerms LNT n ts v s) =
+               substituteTerms LNN n (LNT2LNN_terms n ts) v 
+                 (LNT2LNN_term s)); simpl.
+  - intro n; destruct (eq_nat_dec v n); reflexivity.
+  - intros f t0 H; rewrite H; reflexivity.
+  - reflexivity. 
+  - intros n t0 H t1 H0; now rewrite H, H0.
 Qed.
 
-Lemma LNT2LNN_freeVarTerm :
- forall t : Term, freeVarTerm LNN (LNT2LNN_term t) = freeVarTerm LNT t.
+Lemma LNT2LNN_freeVarTerm ( t : Term):
+  freeVarTerm LNN (LNT2LNN_term t) = freeVarTerm LNT t.
 Proof.
-intros.
-elim t using
- Term_Terms_ind
-  with
+  elim t using
+    Term_Terms_ind
+    with
     (P0 := fun (n : nat) (ts : fol.Terms LNT n) =>
-           freeVarTerms LNN n (LNT2LNN_terms n ts) = freeVarTerms LNT n ts);
- simpl in |- *; intros.
-reflexivity.
-transitivity
- (freeVarTerms LNN (LNTFunctionArity f)
-    (LNT2LNN_terms (LNTFunctionArity f) t0)).
-reflexivity.
-rewrite H.
-reflexivity.
-reflexivity.
-transitivity
- (freeVarTerm LNN (LNT2LNN_term t0) ++
-  freeVarTerms LNN n (LNT2LNN_terms n t1)).
-reflexivity.
-rewrite H.
-rewrite H0.
-reflexivity.
+             freeVarTerms _ n (LNT2LNN_terms n ts) = freeVarTerms LNT n ts);
+    simpl in |- *.  
+  - reflexivity.
+  - intros f t0 H; transitivity
+                     (freeVarTerms LNN (LNTFunctionArity f)
+                        (LNT2LNN_terms (LNTFunctionArity f) t0)).
+    + reflexivity.
+    + now rewrite H.
+  - reflexivity.
+  - intros n t0 H t1 H0; transitivity
+                           (freeVarTerm LNN (LNT2LNN_term t0) ++
+                              freeVarTerms LNN n (LNT2LNN_terms n t1)).
+    + reflexivity.
+    + now rewrite H, H0.
 Qed.
 
-Lemma LNT2LNN_freeVarFormula :
- forall f : Formula,
- freeVarFormula LNN (LNT2LNN_formula f) = freeVarFormula LNT f.
+Lemma LNT2LNN_freeVarFormula (f : Formula):
+  freeVarFormula LNN (LNT2LNN_formula f) = freeVarFormula LNT f.
 Proof.
-intros.
-induction f as [t t0| r t| f1 Hrecf1 f0 Hrecf0| f Hrecf| n f Hrecf];
- simpl in |- *.
-repeat rewrite LNT2LNN_freeVarTerm.
-reflexivity.
-induction r.
-rewrite Hrecf1.
-rewrite Hrecf0.
-reflexivity.
-assumption.
-rewrite Hrecf.
-reflexivity.
+  induction f as [t t0| r t| f1 Hrecf1 f0 Hrecf0| f Hrecf| n f Hrecf];
+    simpl in |- *.
+  - repeat rewrite LNT2LNN_freeVarTerm; reflexivity.
+  - destruct r.
+  - now rewrite Hrecf1,  Hrecf0.
+  - assumption.
+  - now rewrite Hrecf.
 Qed.
 
 Lemma LNT2LNN_subFormula :
- forall (f : Formula) (v : nat) (s : Term),
- LNT2LNN_formula (substituteFormula LNT f v s) =
- substituteFormula LNN (LNT2LNN_formula f) v (LNT2LNN_term s).
+  forall (f : Formula) (v : nat) (s : Term),
+    LNT2LNN_formula (substituteFormula LNT f v s) =
+      substituteFormula LNN (LNT2LNN_formula f) v (LNT2LNN_term s).
 Proof.
-intro.
-elim f using Formula_depth_ind2; simpl in |- *; intros.
-repeat rewrite LNT2LNN_subTerm.
-reflexivity.
-induction r.
-rewrite (subFormulaImp LNT).
-simpl in |- *.
-rewrite H.
-rewrite H0.
-rewrite (subFormulaImp LNN).
-reflexivity.
-rewrite (subFormulaNot LNT).
-simpl in |- *.
-rewrite H.
-rewrite (subFormulaNot LNN).
-reflexivity.
-rewrite (subFormulaForall LNT).
-rewrite (subFormulaForall LNN).
-induction (eq_nat_dec v v0).
-reflexivity.
-rewrite LNT2LNN_freeVarTerm.
-induction (In_dec eq_nat_dec v (freeVarTerm LNT s)).
-simpl in |- *.
-repeat rewrite H.
-simpl in |- *.
-rewrite LNT2LNN_freeVarFormula.
-reflexivity.
-apply depthForall.
-eapply eqDepth.
-symmetry  in |- *; rewrite subFormulaDepth; symmetry  in |- *.
-reflexivity.
-apply depthForall.
-simpl in |- *.
-rewrite H.
-reflexivity.
-apply depthForall.
+  intro f.
+  elim f using Formula_depth_ind2; simpl in |- *.
+  - intros t t0 v s; now repeat rewrite LNT2LNN_subTerm.
+  - intro r; destruct r.
+  - intros f0 H f1 H0 v s; rewrite (subFormulaImp LNT).
+    simpl; now rewrite H, H0, (subFormulaImp LNN).
+  - intros f0 H n H0; rewrite (subFormulaNot LNT); simpl. 
+    now rewrite H, (subFormulaNot LNN).
+  - intros v a H v0 s; 
+      rewrite (subFormulaForall LNT), (subFormulaForall LNN).
+    destruct (eq_nat_dec v v0) as [e | n].
+    + reflexivity.
+    + rewrite LNT2LNN_freeVarTerm.
+      destruct (In_dec eq_nat_dec v (freeVarTerm LNT s)) as [i | i].
+      * simpl; repeat rewrite H; simpl. 
+        -- now rewrite LNT2LNN_freeVarFormula.
+        -- apply depthForall.
+        -- eapply eqDepth.
+           ++ symmetry; rewrite subFormulaDepth; symmetry.
+              reflexivity.
+           ++ apply depthForall.
+      * simpl; rewrite H.
+        -- reflexivity.
+        -- apply depthForall.
 Qed.
 
 Section Translate_Proof.
@@ -691,307 +549,248 @@ Variable V : System.
 
 Hypothesis
   AxiomsOK :
-    forall f : fol.Formula LNN,
-    mem _ U f ->  
+    forall f : fol.Formula LNN, mem _ U f ->  
     exists Axm : Formulas,
     (exists prf : Prf LNT Axm (LNN2LNT_formula f),
        (forall g : Formula, In g Axm -> mem _ V g)) /\
-    forall v, In v (freeVarListFormula LNT Axm) -> (In v (freeVarFormula LNN f)).
+    forall v, In v (freeVarListFormula LNT Axm) -> 
+              (In v (freeVarFormula LNN f)).
 
-Lemma translatePrf : forall f,
+Lemma translatePrf f : 
  forall axm, Prf LNN axm f -> 
   (forall g, In g axm -> mem _ U g) ->
   exists Axm : Formulas,
     (exists prf : Prf LNT Axm (LNN2LNT_formula f),
        (forall g : Formula, In g Axm -> mem _ V g)) /\
-    forall v, In v (freeVarListFormula LNT Axm) -> (In v (freeVarListFormula LNN axm)).
+    forall v, In v (freeVarListFormula LNT Axm) -> 
+              (In v (freeVarListFormula LNN axm)).
 Proof.
-intros f x x0 H.
-induction x0
- as
-  [A|
-   Axm1 Axm2 A B x0_1 Hrecx0_1 x0_0 Hrecx0_0|
-   Axm A v n x0 Hrecx0|
-   A B|
-   A B C|
-   A B|
-   A v t|
-   A v n|
-   A B v|
-   |
-   |
-   |
-   R|
-   f].
-destruct (AxiomsOK A).
-auto with *.
-exists x.
-destruct H0.
-split.
-apply H0.
-intros.
-simpl.
-rewrite <- app_nil_end.
-apply H1.
-apply H2.
-assert (forall g : fol.Formula LNN,
-            In g Axm2 -> mem (fol.Formula LNN) U g).
-intros.
-apply H.
-apply in_or_app.
-auto.
-assert (forall g : fol.Formula LNN,
-            In g Axm1 -> mem (fol.Formula LNN) U g).
-intros.
-apply H.
-apply in_or_app.
-auto.
-destruct (Hrecx0_0 H0) as [x [[x0 I0] Z0]].
-destruct (Hrecx0_1 H1) as [x1 [[x2 I1] Z1]].
-clear H0 H1.
-rename I0 into H0.
-rename I1 into H1.
-exists (x1 ++ x).
-simpl in x2.
-split.
-exists (MP LNT _ _ _ _ x2 x0).
-intros.
-induction (in_app_or _ _ _ H2); auto.
-intros.
-rewrite freeVarListFormulaApp.
-rewrite freeVarListFormulaApp in H2.
-apply in_or_app.
-destruct (in_app_or _ _ _ H2);
-auto with *.
-destruct (Hrecx0 H) as [x [[x1 H0] Z]].
-exists x.
-assert (~ In v (freeVarListFormula LNT x)).
-firstorder.
-split.
-exists (GEN LNT _ _ _ H1 x1).
-assumption.
-assumption.
-exists (nil (A:=Formula)).
-split.
-exists (IMP1 LNT (LNN2LNT_formula A) (LNN2LNT_formula B)).
-contradiction.
-contradiction.
-exists (nil (A:=Formula)).
-split.
-exists (IMP2 LNT (LNN2LNT_formula A) (LNN2LNT_formula B) (LNN2LNT_formula C)).
-contradiction.
-contradiction.
-exists (nil (A:=Formula)).
-split.
-exists (CP LNT (LNN2LNT_formula A) (LNN2LNT_formula B)).
-contradiction.
-contradiction.
-assert (SysPrf (Empty_set _) (LNN2LNT_formula (fol.impH LNN (fol.forallH LNN v A) (substituteFormula LNN A v t)))).
-simpl in |- *.
-apply
- impE
-  with
-    (impH (forallH v (LNN2LNT_formula A))
-       (substituteFormula LNT (LNN2LNT_formula A) v (LNN2LNT_term t))).
-apply iffE1.
-apply (reduceImp LNT).
-apply iffRefl.
-apply iffSym.
-apply LNN2LNT_subFormula.
-exists (nil (A:=Formula)).
-exists (FA1 LNT (LNN2LNT_formula A) v (LNN2LNT_term t)).
-contradiction.
-destruct H0.
-exists x.
-split.
-destruct H0.
-exists x0.
-intros.
-elim (H0 g H1).
-intros.
-destruct H0.
-destruct x.
-assumption.
-assert (In f (f::x)).
-auto with *.
-elim (H0 f H2).
-exists (nil (A:=Formula)).
-assert (~ In v (freeVarFormula LNT (LNN2LNT_formula A))).
-unfold not in |- *; intros; elim n.
-apply LNN2LNT_freeVarFormula1.
-auto.
-split.
-exists (FA2 LNT (LNN2LNT_formula A) v H0).
-contradiction.
-contradiction.
-exists (nil (A:=Formula)).
-split.
-exists (FA3 LNT (LNN2LNT_formula A) (LNN2LNT_formula B) v).
-contradiction.
-contradiction.
-exists (nil (A:=Formula)).
-split.
-exists (EQ1 LNT).
-contradiction.
-contradiction.
-exists (nil (A:=Formula)).
-split.
-exists (EQ2 LNT).
-contradiction.
-contradiction.
-exists (nil (A:=Formula)).
-split.
-exists (EQ3 LNT).
-contradiction.
-contradiction.
-assert (SysPrf (Empty_set _) (LNN2LNT_formula (AxmEq4 LNN R))).
-induction R.
-simpl in |- *.
-repeat apply impI.
-unfold notH, impH in |- *.
-apply
- impE
-  with
-    (iffH
-       (translateLT
-          (Tcons LNN 1 (fol.var LNN 2)
-             (Tcons LNN 0 (fol.var LNN 0) (Tnil LNN))))
-       (translateLT
-          (Tcons LNN 1 (fol.var LNN 3)
-             (Tcons LNN 0 (fol.var LNN 1) (Tnil LNN))))).
-apply impRefl.
-repeat rewrite translateLT1.
-simpl in |- *.
-unfold newVar in |- *.
-simpl in |- *.
-apply
- impE
-  with
-    (iffH (existH 3 (equal (Plus (var 2) (Succ (var 3))) (var 0)))
-       (existH 4 (equal (Plus (var 3) (Succ (var 4))) (var 1)))).
-apply impRefl.
-eapply
- iffTrans
+  intros x x0 H; induction x0
+    as
+    [A|
+      Axm1 Axm2 A B x0_1 Hrecx0_1 x0_0 Hrecx0_0|
+      Axm A v n x0 Hrecx0|
+      A B|
+      A B C|
+      A B|
+      A v t|
+      A v n|
+      A B v|
+    |
+    |
+    |
+      R|
+      f].
+  - destruct (AxiomsOK A). 
+    + apply H; now constructor. 
+    + exists x; destruct H0 as [H0 H1].
+      split.
+      * apply H0.
+      * intros v H2; simpl; rewrite <- app_nil_end.
+        apply H1, H2.
+  - assert (H0: forall g : fol.Formula LNN,
+               In g Axm2 -> mem (fol.Formula LNN) U g).
+    { intros g H0; apply H; apply in_or_app; now right.
+    } 
+    assert (H1: forall g : fol.Formula LNN,
+               In g Axm1 -> mem (fol.Formula LNN) U g).
+    { intros g H1; apply H; apply in_or_app; now left. }
+    destruct (Hrecx0_0 H0) as [x [[x0 I0] Z0]].
+    destruct (Hrecx0_1 H1) as [x1 [[x2 I1] Z1]].
+    clear H0 H1; rename I0 into H0; rename I1 into H1.
+    exists (x1 ++ x);  simpl in x2; split.
+    + exists (MP LNT _ _ _ _ x2 x0).
+      intros g H2; induction (in_app_or _ _ _ H2); auto.
+    + intros v H2;  rewrite freeVarListFormulaApp.
+      rewrite freeVarListFormulaApp in H2;  apply in_or_app.
+      destruct (in_app_or _ _ _ H2); auto with *.
+  - destruct (Hrecx0 H) as [x [[x1 H0] Z]]; exists x.
+    assert (H1: ~ In v (freeVarListFormula LNT x)) by firstorder.
+    split.
+    + exists (GEN LNT _ _ _ H1 x1) ; assumption.
+    + assumption.
+  - exists (nil (A:=Formula)); split.
+    + exists (IMP1 LNT (LNN2LNT_formula A) (LNN2LNT_formula B)).
+      contradiction.
+    + contradiction.
+  - exists (nil (A:=Formula)); split.
+    * exists (IMP2 LNT (LNN2LNT_formula A) (LNN2LNT_formula B) 
+                (LNN2LNT_formula C)); contradiction.
+    * contradiction.
+  - exists (nil (A:=Formula)); split.
+    * exists (CP LNT (LNN2LNT_formula A) (LNN2LNT_formula B)).
+      contradiction.
+    * contradiction.
+  - assert (H0: SysPrf (Empty_set _)
+                  (LNN2LNT_formula 
+                     (fol.impH LNN (fol.forallH LNN v A) 
+                        (substituteFormula LNN A v t)))).
+    { simpl in |- *.
+      apply impE with
+        (impH (forallH v (LNN2LNT_formula A))
+           (substituteFormula LNT (LNN2LNT_formula A) v 
+              (LNN2LNT_term t))).
+      apply iffE1.
+      apply (reduceImp LNT).
+      apply iffRefl.
+      apply iffSym.
+      apply LNN2LNT_subFormula.
+      exists (nil (A:=Formula)).
+      exists (FA1 LNT (LNN2LNT_formula A) v (LNN2LNT_term t)).
+      contradiction.
+    }
+    destruct H0 as [x H0]; exists x; split.
+    + destruct H0 as [x0 H0]; exists x0.
+      intros g H1; elim (H0 g H1).
+    + intros v0 H1; destruct H0.
+      * destruct x. 
+        -- assumption.
+        -- assert (H2: In f (f::x)) by  auto with *.
+           elim (H0 f H2).
+  - exists (nil (A:=Formula)).
+    assert (H0: ~ In v (freeVarFormula LNT (LNN2LNT_formula A))).
+    { unfold not in |- *; intros; elim n.
+      apply LNN2LNT_freeVarFormula1.
+      auto.
+    } split.
+    + exists (FA2 LNT (LNN2LNT_formula A) v H0); contradiction.
+    + contradiction.
+  - exists (nil (A:=Formula)); split.
+    + exists (FA3 LNT (LNN2LNT_formula A) (LNN2LNT_formula B) v);
+        contradiction.
+    + contradiction.
+  - exists (nil (A:=Formula)); split.
+    + exists (EQ1 LNT); contradiction.
+    + contradiction.
+  - exists (nil (A:=Formula)); split.
+    + exists (EQ2 LNT); contradiction.
+    + contradiction.
+  - exists (nil (A:=Formula)); split.
+    + exists (EQ3 LNT); contradiction.
+    + contradiction.
+  - assert (H0: SysPrf (Empty_set _) (LNN2LNT_formula (AxmEq4 LNN R))).
+    { induction R; simpl; repeat apply impI.
+      unfold notH, impH ; apply impE
+        with
+        (iffH
+           (translateLT
+              (Tcons LNN 1 (fol.var LNN 2)
+                 (Tcons LNN 0 (fol.var LNN 0) (Tnil LNN))))
+           (translateLT
+              (Tcons LNN 1 (fol.var LNN 3)
+                 (Tcons LNN 0 (fol.var LNN 1) (Tnil LNN))))).
+      - apply impRefl.
+      - repeat rewrite translateLT1; simpl; unfold newVar; simpl.  
+        apply impE 
           with
-          (existH 4
-             (substituteFormula LNT
-                (equal (Plus (var 2) (Succ (var 3))) (var 0)) 3 
-                (var 4))).
-apply (rebindExist LNT).
-simpl in |- *.
-unfold not in |- *; intros.
-decompose sum H0.
-discriminate H1.
-discriminate H2.
-apply (reduceExist LNT).
-unfold not in |- *; intros.
-induction H0 as (x, H0); induction H0 as (H0, H1).
-induction H1 as [x H1| x H1]; [ induction H1 as [x H1| x H1] | induction H1 ].
-elim H1.
-induction H1.
-simpl in H0.
-decompose sum H0.
-discriminate H1.
-discriminate H2.
-simpl in H0.
-decompose sum H0.
-discriminate H1.
-discriminate H2.
-repeat rewrite (subFormulaEqual LNT).
-simpl in |- *.
-apply iffI.
-apply impI.
-apply eqTrans with (var 0).
-apply eqTrans with (Plus (var 2) (Succ (var 4))).
-apply eqPlus.
-apply eqSym.
-apply Axm.
-left.
-left.
-right.
-constructor.
-apply eqRefl.
-apply Axm.
-right; constructor.
-apply Axm; left; right; constructor.
-apply impI.
-apply eqTrans with (var 1).
-apply eqTrans with (Plus (var 3) (Succ (var 4))).
-fold (Succ (var 4)) in |- *.
-fold (Plus (fol.var LNT 2) (Succ (var 4))) in |- *.
-apply eqPlus.
-apply Axm.
-left.
-left.
-right.
-constructor.
-apply eqRefl.
-apply Axm.
-right; constructor.
-apply eqSym.
-apply Axm; left; right; constructor.
-destruct H0.
-exists x.
-destruct H0.
-split.
-exists x0.
-intros.
-elim (H0 g H1).
-intros.
-destruct x.
-assumption.
-assert (In f (f::x)).
-auto with *.
-elim (H0 _ H2).
-replace (LNN2LNT_formula (AxmEq5 LNN f)) with (AxmEq5 LNT f).
-exists (nil (A:=Formula)).
-split.
-exists (EQ5 LNT f).
-contradiction.
-contradiction.
-induction f; reflexivity.
+          (iffH (existH 3 (equal (Plus (var 2) (Succ (var 3))) (var 0)))
+             (existH 4 (equal (Plus (var 3) (Succ (var 4))) (var 1)))).
+        + apply impRefl.
+        + eapply iffTrans with
+            (existH 4
+               (substituteFormula LNT
+                  (equal (Plus (var 2) (Succ (var 3))) (var 0)) 3 
+                  (var 4))).
+          * apply (rebindExist LNT).
+            simpl in |- *. intro H0; decompose sum H0.
+            -- discriminate H1.
+            -- discriminate H2.
+          * apply (reduceExist LNT).
+            intros (x, (H0, H1)).
+            destruct H1 as [x H1| x H1]; [ destruct H1 as [x H1| x H1] | 
+                                           destruct H1 ].
+            -- elim H1.
+            -- induction H1.
+               simpl in H0.
+               decompose sum H0.
+               discriminate H1.
+               discriminate H2.
+            -- simpl in H0; decompose sum H0.
+               discriminate H1.
+               discriminate H2.
+            -- repeat rewrite (subFormulaEqual LNT); simpl.
+               apply iffI.
+               ++ apply impI.
+                  apply eqTrans with (var 0).
+                  ** apply eqTrans with (Plus (var 2) (Succ (var 4))).
+                     apply eqPlus.
+                     apply eqSym.
+                     apply Axm.
+                     left.
+                     left.
+                     right.
+                     constructor.
+                     apply eqRefl.
+                     apply Axm.
+                     right; constructor.
+                  ** apply Axm; left; right; constructor.
+               ++ apply impI.
+                  apply eqTrans with (var 1).
+                  **  apply eqTrans with (Plus (var 3) (Succ (var 4))).
+                      fold (Succ (var 4)) in |- *.
+                      fold (Plus (fol.var LNT 2) (Succ (var 4))) in |- *.
+                      apply eqPlus.
+                      apply Axm.
+                      left.
+                      left.
+                      right.
+                      constructor.
+                      apply eqRefl.
+                      apply Axm.
+                      right; constructor.
+                  ** apply eqSym.
+                     apply Axm; left; right; constructor.
+    }    
+    destruct H0 as [x H0]; exists x.
+    destruct H0 as [x0 H0]; split.
+    + exists x0; intros g H1; elim (H0 g H1).
+    + intros v H1; destruct x.
+      * assumption.
+      * assert (H2: In f (f::x)) by auto with *.
+        elim (H0 _ H2).
+  - replace (LNN2LNT_formula (AxmEq5 LNN f)) with (AxmEq5 LNT f).
+    + exists (nil (A:=Formula)); split.
+      * exists (EQ5 LNT f); contradiction.
+      * contradiction.
+    + induction f; reflexivity.
 Qed.
 
 End Translate_Proof.
 
-Lemma translateProof
-     : forall (U : fol.System LNN) (V : System),
-       ClosedSystem LNT V ->
-       (forall f : fol.Formula LNN,
+Lemma translateProof (U : fol.System LNN) (V : System):
+    ClosedSystem LNT V ->
+    (forall f : fol.Formula LNN,
         mem (fol.Formula LNN) U f -> SysPrf V (LNN2LNT_formula f)) ->
-       forall f : fol.Formula LNN,
-       folProof.SysPrf LNN U f -> SysPrf V (LNN2LNT_formula f).
+    forall f : fol.Formula LNN,
+      folProof.SysPrf LNN U f -> SysPrf V (LNN2LNT_formula f).
 Proof.
-intros.
-destruct H1.
-assert (forall f : fol.Formula LNN,
-        mem (fol.Formula LNN) U f ->
-        exists Axm : Formulas,
-          ex
-            (fun _ : Prf LNT Axm (LNN2LNT_formula f) =>
-             forall g : Formula, In g Axm -> mem (fol.Formula LNT) V g) /\
-          (forall v : nat,
-           In v (freeVarListFormula LNT Axm) -> In v (freeVarFormula LNN f))).
-intros.
-destruct (H0 f0 H2).
-exists x0.
-split.
-apply H3.
-intros.
-destruct H3.
-clear x1.
-induction x0.
-elim H4.
-destruct (in_app_or _ _ _ H4).
-elim H with v a.
-apply H3.
-auto with *.
-assumption.
-apply IHx0.
-firstorder.
-apply H5.
-destruct H1.
-destruct (translatePrf U V H2 f x x0 H1).
-exists x1.
-tauto.
+  intros H H0 f [x H1]. 
+  assert (H2: forall f : fol.Formula LNN,
+             mem (fol.Formula LNN) U f ->
+             exists Axm : Formulas,
+               ex
+                 (fun _ : Prf LNT Axm (LNN2LNT_formula f) =>
+                    forall g : Formula, In g Axm -> 
+                                        mem (fol.Formula LNT) V g) /\
+                 (forall v : nat,
+                     In v (freeVarListFormula LNT Axm) -> 
+                     In v (freeVarFormula LNN f))).
+  { intros f0 H2; destruct (H0 f0 H2) as [x0 H3]. 
+    exists x0; split.
+    - apply H3.
+    - intros v H4; destruct H3.
+      clear x1; induction x0.
+      + elim H4.
+      + destruct (in_app_or _ _ _ H4) as [H5 | H5].
+        *  elim H with v a.
+           apply H3.
+           auto with *.
+           assumption.
+        * apply IHx0.
+          firstorder.
+          apply H5.
+  }   
+  destruct H1.
+  destruct (translatePrf U V H2 f x x0 H1).
+  exists x1; tauto.
 Qed.
